@prefix : <https://www.w3.org/2019/json-schema#> .
@prefix dc: <http://purl.org/dc/elements/1.1/> .
@prefix vs: <http://www.w3.org/2003/06/sw-vocab-status/ns#> .
@prefix owl: <http://www.w3.org/2002/07/owl#> .
@prefix rdf: <http://www.w3.org/1999/02/22-rdf-syntax-ns#> .
@prefix xml: <http://www.w3.org/XML/1998/namespace> .
@prefix xsd: <http://www.w3.org/2001/XMLSchema#> .
@prefix foaf: <http://xmlns.com/foaf/0.1/> .
@prefix prov: <http://www.w3.org/ns/prov#> .
@prefix rdfs: <http://www.w3.org/2000/01/rdf-schema#> .
@prefix vann: <http://purl.org/vocab/vann/> .
@prefix dcterms: <http://purl.org/dc/terms/> .

<https://www.w3.org/2019/json-schema#> rdf:type owl:Ontology ;
                                    
                                    owl:versionInfo "0.5.0" ;
                                    
                                    rdfs:comment "Module for data schema specifications, part of the W3C Web of Things (WoT) Thing Description model"@en ;
                                    
                                    vann:preferredNamespacePrefix "jsonschema" ;
                                    
                                    vann:preferredNamespaceUri "https://www.w3.org/2019/json-schema#" ;
                                    
                                    dc:title "JSON Schema in RDF"@en ;
                                    
                                    dcterms:license <http://purl.org/NET/rdflicense/cc-by4.0> ;
                                    
                                    dc:publisher <https://www.w3.org/WoT/WG/> ;
                                    
                                    dcterms:creator <mailto:victor.charpenay@siemens.com> .


#################################################################
#
#    Object Properties
#
#################################################################


###  https://www.w3.org/2019/json-schema#items

<https://www.w3.org/2019/json-schema#items> rdf:type owl:ObjectProperty ;
                                         
                                         rdfs:label "items" ;
                                         
                                         rdfs:comment "Used to define the characteristics of an array."@en.



###  https://www.w3.org/2019/json-schema#properties

<https://www.w3.org/2019/json-schema#properties> rdf:type owl:ObjectProperty ;
                                              
                                              rdfs:label "properties" ;
                                              
                                              rdfs:comment "Data schema nested definitions"@en .





#################################################################
#
#    Data properties
#
#################################################################


###  https://www.w3.org/2019/json-schema#const

<https://www.w3.org/2019/json-schema#const> rdf:type owl:DatatypeProperty ;
                                         
                                         rdfs:label "const" ;
                                         
                                         rdfs:comment "Provides a constant value."@en .



###  https://www.w3.org/2019/json-schema#enum

<https://www.w3.org/2019/json-schema#enum> rdf:type owl:DatatypeProperty ;
                                        
                                        rdfs:label "enum" ;
                                        
                                        rdfs:comment "Restricted set of values provided as an array."@en .



###  https://www.w3.org/2019/json-schema#oneOf

<https://www.w3.org/2019/json-schema#oneOf> rdf:type owl:DatatypeProperty ;
                                        
                                        rdfs:label "oneOf" ;
                                        
                                        rdfs:comment "Used to ensure that the data is valid against one of the specified schemas in the array."@en .




###  https://www.w3.org/2019/json-schema#maxItems

<https://www.w3.org/2019/json-schema#maxItems> rdf:type owl:DatatypeProperty ;
                                            
                                            rdfs:label "maxItems" ;
                                            
                                            rdfs:comment "Defines the maximum number of items that have to be in the array."@en .



###  https://www.w3.org/2019/json-schema#maximum

<https://www.w3.org/2019/json-schema#maximum> rdf:type owl:DatatypeProperty ;
                                           
                                           rdfs:label "maximum" ;
                                           
                                           rdfs:comment "Specifies a maximum numeric value. Only applicable for associated number or integer types."@en ;
                                           
                                           rdfs:seeAlso <http://schema.org/maxValue> .



###  https://www.w3.org/2019/json-schema#minItems

<https://www.w3.org/2019/json-schema#minItems> rdf:type owl:DatatypeProperty ;
                                            
                                            rdfs:label "minItems" ;
                                            
                                            rdfs:comment "Defines the minimum number of items that have to be in the array."@en .



###  https://www.w3.org/2019/json-schema#minimum

<https://www.w3.org/2019/json-schema#minimum> rdf:type owl:DatatypeProperty ;
                                           
                                           rdfs:label "minimum" ;
                                           
                                           rdfs:comment "Specifies a minimum numeric value. Only applicable for associated number or integer types."@en ;
                                           
                                           rdfs:seeAlso <http://schema.org/minValue> .



###  https://www.w3.org/2019/json-schema#required

<https://www.w3.org/2019/json-schema#required> rdf:type owl:DatatypeProperty ;
                                            
                                            rdfs:label "required" ;
                                            
                                            rdfs:comment "Defines which members of the object type are mandatory."@en .


###  https://www.w3.org/2019/json-schema#readOnly

<https://www.w3.org/2019/json-schema#readOnly> rdf:type owl:DatatypeProperty ;
                                            
                                            rdfs:label "readOnly" ;
                                            
                                            rdfs:comment "Boolean value that is a hint to indicate whether a property interaction / value is read only (=true) or not (=false)"@en .

 <https://www.w3.org/2019/json-schema#format> rdf:type owl:DatatypeProperty ;
                                            
                                            rdfs:label "format" ;
                                            
                                            rdfs:comment "Defines format pattern validation on certain kinds of string values. It is open to use pattern values that may originate from JSON schema presets (e.g., date/time, email, URL) or other (custom-based) definitions."@en .                                           
                                            
###  https://www.w3.org/2019/json-schema#writeOnly

<https://www.w3.org/2019/json-schema#writeOnly> rdf:type owl:DatatypeProperty ;
                                            
                                            rdfs:label "writeOnly" ;
                                            
                                            rdfs:comment "Boolean value that is a hint to indicate whether a property interaction / value is write only (=true) or not (=false)"@en .

###  https://www.w3.org/2019/json-schema#type

<https://www.w3.org/2019/json-schema#type> rdf:type owl:DatatypeProperty ;
                                        
                                        rdfs:label "type" ;
                                        
                                        rdfs:comment "Assignment of JSON-based data types compatible with JSON Schema (one of boolean, integer, number, string, object, array, or null)." .





#################################################################
#
#    Classes
#
#################################################################


###  https://www.w3.org/2019/json-schema#ArraySchema

<https://www.w3.org/2019/json-schema#ArraySchema> rdf:type owl:Class ;
                                               
                                               rdfs:subClassOf <https://www.w3.org/2019/json-schema#DataSchema> ;
                                               
                                               rdfs:comment "A JSON array specification (\"type\": \"array\")."@en .



###  https://www.w3.org/2019/json-schema#BooleanSchema

<https://www.w3.org/2019/json-schema#BooleanSchema> rdf:type owl:Class ;
                                                 
                                                 rdfs:subClassOf <https://www.w3.org/2019/json-schema#DataSchema> ;
                                                 
                                                 rdfs:comment "A JSON boolean value specification (\"type\": \"boolean\")."@en .



###  https://www.w3.org/2019/json-schema#NullSchema

<https://www.w3.org/2019/json-schema#NullSchema> rdf:type owl:Class ;
                                                 
                                                 rdfs:subClassOf <https://www.w3.org/2019/json-schema#DataSchema> ;
                                                 
                                                 rdfs:comment "A JSON null value specification (\"type\": \"null\"). If the type of null then it has only one acceptable value, namely null. E.g., it can be used as part of oneOf declaration, where it is used to indicate, that a data schema can also be null."@en .



###  https://www.w3.org/2019/json-schema#DataSchema

<https://www.w3.org/2019/json-schema#DataSchema> rdf:type owl:Class ;
                                                
                                              rdfs:comment "A JSON specification." .



###  https://www.w3.org/2019/json-schema#IntegerSchema

<https://www.w3.org/2019/json-schema#IntegerSchema> rdf:type owl:Class ;
                                                 
                                                 rdfs:subClassOf <https://www.w3.org/2019/json-schema#DataSchema> ;
                                                 
                                                 rdfs:comment "A JSON integer value specification, that is, numbers without a fractional part (\"type\": \"integer\")."@en .



###  https://www.w3.org/2019/json-schema#NumberSchema

<https://www.w3.org/2019/json-schema#NumberSchema> rdf:type owl:Class ;
                                                
                                                rdfs:subClassOf <https://www.w3.org/2019/json-schema#DataSchema> ;
                                                
                                                rdfs:comment "A JSON number value specification (\"type\": \"number\")."@en .



###  https://www.w3.org/2019/json-schema#ObjectSchema

<https://www.w3.org/2019/json-schema#ObjectSchema> rdf:type owl:Class ;
                                                
                                                rdfs:subClassOf <https://www.w3.org/2019/json-schema#DataSchema> ;
                                                
                                                rdfs:comment "A JSON object specification (\"type\": \"object\")."@en .



###  https://www.w3.org/2019/json-schema#StringSchema

<https://www.w3.org/2019/json-schema#StringSchema> rdf:type owl:Class ;
                                                
                                                rdfs:subClassOf <https://www.w3.org/2019/json-schema#DataSchema> ;
                                                
                                                rdfs:comment "A JSON string value specification (\"type\": \"string\")."@en .




###  Generated by the OWL API (version 3.4.2) http://owlapi.sourceforge.net

